$$
\begin{align*}
a) &\,\frac{2}{\sqrt{ 3 }}&b)& \frac{1}{\sqrt{ 3 }}&c)& \frac{3}{\sqrt{ 2 }}&d)& \frac{5}{\sqrt{ 7 }} &e)& \frac{7}{\sqrt{ 2 }}\\
f)& \frac{\sqrt{ 2 }}{\sqrt{ 3 }}&g)& \frac{\sqrt{ 3 }}{\sqrt{ 7 }}&h)& \frac{\sqrt{ 2 }}{\sqrt{ 18 }}& i)& \frac{\sqrt{ 5 }}{\sqrt{ 10 }}& j)& \frac{\sqrt{ 7 }}{\sqrt{ 12 }}
\end{align*}
$$


$$
\begin{align*}
a)&\\
&=\frac{2}{\sqrt{ 3 }}\cdot \frac{\sqrt{ 3 }}{\sqrt{ 3 }}\\
&=\frac{2\sqrt{ 3}}{\sqrt{ 3\cdot 3 }}\\
&=\frac{2\sqrt{ 3 }}{\sqrt{ 9 }}\\
&=\frac{2\sqrt{ 3 }}{3}\\
\end{align*}
$$
$$
\begin{align*}
b)&\\
&=\frac{1}{\sqrt{ 3 }}\cdot \frac{\sqrt{ 3 }}{\sqrt{ 3 }}\\
&=\frac{1\sqrt{ 3}}{\sqrt{ 3\cdot 3 }}\\
&=\frac{\sqrt{ 3 }}{\sqrt{ 9 }}\\
&=\frac{\sqrt{ 3 }}{3}\\
\end{align*}
$$
$$
\begin{align*}
c)&\\
&=\frac{3}{\sqrt{ 2 }}\cdot \frac{\sqrt{ 2 }}{\sqrt{ 2 }}\\
&=\frac{3\sqrt{ 2}}{\sqrt{ 2\cdot 2 }}\\
&=\frac{3\sqrt{ 2 }}{\sqrt{ 4 }}\\
&=\frac{3\sqrt{ 2 }}{2}\\
\end{align*}
$$
$$
\begin{align*}
d)&\\
&=\frac{5}{\sqrt{ 2 }}\cdot \frac{\sqrt{ 7 }}{\sqrt{ 7 }}\\
&=\frac{5\sqrt{ 7}}{\sqrt{ 7\cdot 7 }}\\
&=\frac{5\sqrt{ 7 }}{\sqrt{ 49 }}\\
&=\frac{5\sqrt{ 7 }}{7}\\
\end{align*}
$$
$$
\begin{align*}
e)&\\
&=\frac{7}{\sqrt{ 2 }}\cdot \frac{\sqrt{ 2 }}{\sqrt{ 2 }}\\
&=\frac{7\sqrt{ 2}}{\sqrt{ 2\cdot 2 }}\\
&=\frac{7\sqrt{ 2 }}{\sqrt{ 4 }}\\
&=\frac{7\sqrt{ 2 }}{2}\\
\end{align*}
$$
$$
\begin{align*}
f)&\\
&=\frac{\sqrt{ 2 }}{\sqrt{ 3 }}\cdot \frac{\sqrt{ 3 }}{\sqrt{ 3 }}\\
&=\frac{\sqrt{ 2\cdot 3}}{\sqrt{ 3\cdot 3 }}\\
&=\frac{\sqrt{ 6 }}{\sqrt{ 9 }}\\
&=\frac{\sqrt{ 6 }}{3}\\
\end{align*}
$$
$$
\begin{align*}
g)&\\
&=\frac{\sqrt{ 3 }}{\sqrt{ 7 }}\cdot \frac{\sqrt{ 7 }}{\sqrt{ 7 }}\\
&=\frac{\sqrt{ 3\cdot 7}}{\sqrt{ 7\cdot 7 }}\\
&=\frac{\sqrt{ 21 }}{\sqrt{ 49 }}\\
&=\frac{\sqrt{ 21 }}{7}\\
\end{align*}
$$
$$
\begin{align*}
h)&\\
&=\frac{\sqrt{ 2 }}{\sqrt{ 18 }}\cdot \frac{\sqrt{ 18 }}{\sqrt{ 18 }}\\
&=\frac{\sqrt{ 2\cdot 18}}{\sqrt{ 18\cdot 18 }}\\
&=\frac{\sqrt{ 36 }}{\sqrt{ 18^{2} }}\\
&=\frac{\sqrt{6^{2}}}{18}\\
&=\frac{6}{18}\\
&=\frac{1}{3}
\end{align*}
$$
$$
\begin{align*}
i)&\\
&=\frac{\sqrt{ 5 }}{\sqrt{ 10 }}\cdot \frac{\sqrt{ 10 }}{\sqrt{ 10 }}\\
&=\frac{\sqrt{ 5\cdot 10}}{\sqrt{ 10\cdot 10 }}\\
&=\frac{\sqrt{ 50 }}{\sqrt{ 10^{2} }}\\
&=\frac{\sqrt{ 2\cdot 5^{2} }}{10}\\
&=\frac{5\sqrt{ 2 }}{10}\\
&=\frac{\sqrt{ 2 }}{2}
\end{align*}
$$
$$
\begin{align*}
j)&\\
&=\frac{\sqrt{ 7 }}{\sqrt{ 12 }}\cdot \frac{\sqrt{ 12 }}{\sqrt{ 12 }}\\
&=\frac{\sqrt{ 7\cdot 12}}{\sqrt{ 12\cdot 12 }}\\
&=\frac{\sqrt{ 84 }}{\sqrt{ 12^{2} }}\\
&=\frac{\sqrt{ 2^{2} \cdot 21}}{12}\\
&=\frac{2\sqrt{ 21 }}{12}\\
&=\frac{\sqrt{ 21 }}{6}
\end{align*}
$$
$$
\int _{0}^{2}\int _{x^{2}}^{4}\int _{0}^{x^{2}} \, dz  \, dy  \, dx 
$$







$$
\begin{align*}
I=\int e^{2x}\sin(3x) \, dx &\\
u=e^{2x}\qquad du=2e^{2x}\\
dv=\sin(3x)\,dx\qquad v=-\frac{\cos(3x)}{3}\\
I=-\frac{e^{2x}\cos(3x)}{3}+\frac{2}{3} \int e^{2x}\cos(3x) \, dx \\
u=e^{2x}\qquad du=2e^{2x}dx\\
dv=\cos(3x)dx\qquad v=\frac{1}{3}\sin(3x)\\
I=-\frac{e^{2x}\cos(3x)}{3}+\frac{2}{3}\left( \frac{e^{2x}\sin(3x)}{3}-\frac{2}{3} \int e^{2x}\sin(3x) \, dx  \right)\\
I=-\frac{e^{2x}\cos(3x)}{3}+\frac{2e^{2x}\sin(3x)}{9}-\frac{4}{9}\int e^{2x}\sin(3x) \, dx\\
I=-\frac{e^{2x}\cos(3x)}{3}+\frac{2e^{2x}\sin(3x)}{9}-\frac{4}{9}I\\
I+\frac{4}{9}I=-\frac{e^{2x}\cos(3x)}{3}+\frac{2e^{2x}\sin(3x)}{9}\\
\frac{13}{9}I=-\frac{e^{2x}\cos(3x)}{3}+\frac{2e^{2x}\sin(3x)}{9}\\
I=\frac{9}{13}\left( -\frac{e^{2x}\cos(3x)}{3}+\frac{2e^{2x}\sin(3x)}{9} \right)
\end{align*}
$$


$$
\begin{align*}
I=\int e^{2x}\sin(3x) \, dx \\
u=\sin(3x)\qquad du=3\cos(3x)\\
dv=e^{2x}\,dx\qquad v=\frac{1}{2}e^{2x}\\
I=\frac{1}{2}e^{2x}\sin(3x)-\frac{3}{2}\int e^{2x}\cos(3x) \, dx \\
u=\cos(3x)\qquad du=-3\sin(3x)\\
dv=e^{2x}\,dx\qquad v=\frac{1}{2}e^{2x}\\
I=\frac{1}{2}e^{2x}\sin(3x)-\frac{3}{2}\left( \frac{1}{2}e^{2x}\cos(3x)+\frac{3}{2} \int e^{2x}\sin(3x) \, dx  \right)\\
I=\frac{1}{2}e^{2x}\sin(3x)-\frac{3}{4}e^{2x}\cos(3x)-\frac{9}{4}\int e^{2x}\sin(3x) \, dx \\
I=\frac{1}{2}e^{2x}\sin(3x)-\frac{3}{4}e^{2x}\cos(3x)-\frac{9}{4}I\\
I+\frac{9}{4}I=\frac{1}{2}e^{2x}\sin(3x)-\frac{3}{4}e^{2x}\cos(3x)\\
\frac{13}{4}I=\frac{1}{2}e^{2x}\sin(3x)-\frac{3}{4}e^{2x}\cos(3x)\\
I=\frac{4}{13}\left( \frac{1}{2}e^{2x}\sin(3x)-\frac{3}{4}e^{2x}\cos(3x) \right)
\end{align*}
$$